Uniana.v
@@ -14,7 +14,28 @@ Require Util Graph Evaluation Unchanged Disjoint.
 
 Module Uniana.
   Import Util Evaluation.Evaluation Disjoint.Disjoint Unchanged.Unchanged.
-  
+
+  Section uniana.
+
+    Context `(C : redCFG).
+    
+  Parameter branch: Lab -> option Var.
+
+  Definition is_branch br x := branch br = Some x.
+
+  Parameter val_true : Val -> bool.
+
+  Parameter branch_spec :
+    forall p, match branch p with
+         | Some x => exists q q' s r r', q <> q'
+                                   /\ if val_true (s x)
+                                     then eff' (p,s) = Some (q, r)
+                                     else eff' (p,s) = Some (q',r')                                
+         | None => forall q q', p --> q -> p --> q' -> q = q'
+         end.
+
+  Parameter root_no_pred' : forall p, p --> root -> False.
+    
   Parameter init_uni : Var -> Prop.
 
   Definition UniState := Var -> bool.
@@ -30,47 +51,37 @@ Module Uniana.
       eff (p, i, s') = Some (q, j, qs') ->
       uni_state_concr (abs_uni_eff uni) qs qs'.
 
+  Definition Uni := Lab -> Var -> bool.
+
   Definition uni_concr (u : Uni) : Hyper :=
     fun ts => forall t t', ts t -> ts t' ->
                    forall x p i s s', In (p, i, s) (`t) ->
                                  In (p, i, s') (`t') ->
                                  u p x = true -> s x = s' x.
 
-
-
-  Parameter splits : Lab -> (Lab * Lab * Lab * list Var).
-
-  Set Printing All.
-  Parameter splits_spec :
-    forall p br q1 q2 xl,
-      let psplit := splits in
-      
-      <-> (br, q1 ,q2, xl) ∈ splits p
-      
   
-  Definition uni_trans (uni : Uni) (upi : Upi) (unch : Unch) : Uni :=
+  Definition uni_trans (uni : Uni) (unch : Unch) : Uni :=
     fun p
     => if p == root then uni root
       else fun x => ((join_andb
-                     (map (fun spl : Lab * Var
-                           => let (s, x) := spl in
-                             uni s x &&
-                                 join_andb (map (fun spl : Lab * Var
-                                                        => let (s,x) := spl in
-                                                          uni s x
-                                                )
-                                                (preceding_loop_splits p s)
-                                           )
+                     (map (fun spq : Lab * Lab * Lab
+                           => let s := fst (fst spq) in
+                             match (branch s) with
+                             | Some x => uni s x
+                             | None => false
+                             end
                           )
-                          (splits p)))
-                    && (join_andb (map (fun q => abs_uni_eff (uni q) x) (preds p)))
-                    && (join_andb (map (fun q => upi_trans upi uni q p) (preds p)))
+                          (splits p)
+                     )
+                  ) (* the predecessor is only included in split set if p is an exit *)
                  )
-                 || join_orb (map (fun q => (q <>b p) && uni q x && upi_trans upi uni q p)
+                   && (join_andb (map (fun q => abs_uni_eff (uni q) x) (preds p)))
+                 || join_orb (map (fun q => (q <>b p) && uni q x (*&& upi_trans upi uni q p*))
                                  (unch_trans unch p x)).
+  (* unch should be alright now, upi is included in uni *)
 
   Lemma uni_trans_root_inv :
-    forall uni hom unch x, uni_trans uni hom unch root x = uni root x.
+    forall uni unch x, uni_trans uni unch root x = uni root x.
   Proof.
     intros.
     unfold uni_trans.
@@ -79,7 +90,8 @@ Module Uniana.
     exfalso. apply c. reflexivity.
   Qed.
   
-  Lemma branch_eff_eq br s1 s2 x i k k':
+  (*  
+    Lemma branch_eff_eq br s1 s2 x i k k':
     is_branch br x
     -> s1 x = s2 x
     -> eff (br,i,s1) = Some k
@@ -98,20 +110,26 @@ Module Uniana.
     destruct Heff1'. clear Heff2'.
     eapply ivec_det; eauto.
   Qed.
+   *)
         
+  (*
   Lemma splits_is_branch br x p :
     In (br,x) (splits p) -> is_branch br x.
   Proof.
     intro HSsplit.
     eapply splits_spec in HSsplit. unfold DisjointBranch in HSsplit. firstorder.
   Qed.
+   *)
 
+  (*
   Lemma loop_splits_is_branch :
     forall (br : Lab) (x : Var) (p s : Lab), In (br, x) (loop_splits p s) -> is_branch br x.
   Proof.
     intros. eapply loop_splits_spec in H. firstorder.
   Qed.
-  
+   *)
+
+  (*
   Ltac eff_some_k :=
     lazymatch goal with
     | [Htr : Tr ?tq,
@@ -125,8 +143,9 @@ Module Uniana.
         eauto; [|subst tq; simpl_nl;eauto];
         eapply Hpost_incl,In_rcons; tauto
     end.
-
+   *)
   
+  (*
   Lemma is_split_loop_split p0 p q1 q2 br i0 i j1 j2 k l1 l2
     (Hpath1 : TPath (p0,i0) (p,i) ((p, i) :<: (q1, j1) :< l1))
     (Hpath2 : TPath (p0,i0) (p,i) ((p, i) :<: (q2, j2) :< l2))
@@ -134,28 +153,53 @@ Module Uniana.
     (LC_lt : last_common ((q1, j1) :< l1) ((q2, j2) :< l2) (br, k)) :
     (exists x, (br,x) ∈ splits p) \/ exists s x x', (s,x) ∈ splits p /\ (br,x') ∈ preceding_loop_splits p s.
   Admitted.
+   *)
   
-  Lemma disjoint p q1 q2 i j1 j2 s1 s2 r1 r2 (t1 t2 : trace) uni ts l1 l2
+  Lemma uni_same_tag p q i j1 j2 s1 s2 r1 r2 (t1 t2 : trace) uni ts l1 l2
+        (Htr1 : Tr ((p,i,s1) :<: (q,j1,r1) :< l1))
+        (Htr2 : Tr ((p,i,s2) :<: (q,j2,r2) :< l2))
+        (Hpre1 : Prefix ((q,j1,r1) :: l1) (`t1))
+        (Hpre2 : Prefix ((q,j2,r2) :: l2) (`t2))
+        (Hsplit : (join_andb
+                    (map (fun spq : Lab * Lab * Lab
+                            => let s := fst (fst spq) in
+                             match (branch s) with
+                             | Some x => uni s x
+                             | None => false
+                             end
+                           )
+                           (splits p)
+                    )
+                  ) = true)
+        (HCuni : uni_concr uni ts)
+        (Hsem1 : ts t1)
+        (Hsem2 : ts t2)
+    : j2 = j1.
+  Proof.
+    (* use tag_eq_loop_exit *)
+  Admitted.
+
+  Lemma uni_same_lab p q1 q2 i j1 j2 s1 s2 r1 r2 (t1 t2 : trace) uni ts l1 l2
         (Htr1 : Tr ((p,i,s1) :<: (q1,j1,r1) :< l1))
         (Htr2 : Tr ((p,i,s2) :<: (q2,j2,r2) :< l2))
-        (Hpre1 : Prefix l1 (`t1))
-        (Hpre2 : Prefix l2 (`t2))
-        (Hsplit : join_andb
-                    (map
-                       (fun spl : Lab * Var =>
-                          let (s, x) := spl in
-                          uni s x &&
-                              join_andb
-                              (map (fun spl0 : Lab * Var => let (s0, x0) := spl0 in uni s0 x0)
-                                   (preceding_loop_splits p s))) (splits p)) = true)
+        (Hpre1 : Prefix ((q1,j1,r1) :: l1) (`t1))
+        (Hpre2 : Prefix ((q2,j2,r2) :: l2) (`t2))
+        (Hsplit : (join_andb
+                    (map (fun spq : Lab * Lab * Lab
+                            => let s := fst (fst spq) in
+                             match (branch s) with
+                             | Some x => uni s x
+                             | None => false
+                             end
+                           )
+                           (splits p)
+                    )
+                  ) = true)
         (HCuni : uni_concr uni ts)
-        (Hsem1 : sem_trace ts t1)
-        (Hsem2 : sem_trace ts t2) : q2 = q1.
-  Proof.
-
-
-(*  assert (In q2 (preds p)) as Hqpred2 by (eauto using step_conf_implies_edge).*)
-  
+        (Hsem1 : ts t1)
+        (Hsem2 : ts t2)
+    : q2 = q1.
+  Proof.  
   assert (exists (si : Lab * Tag),
              last_common (ne_map fst ((q1,j1,r1) :< l1))
                          (ne_map fst ((q2,j2,r2) :< l2)) si) as [[br k] LC_lt].
@@ -167,137 +211,53 @@ Module Uniana.
   }
   simpl_nl' LC_lt; cbn in LC_lt.
   destruct (q2 == q1) as [ Heq | Hneq ]; [ eauto | exfalso ].
-  eapply is_split_loop_split in LC_lt; eauto.
-  - admit. 
-  - eapply Tr_EPath in Htr1 as [s0 Htr1];[|cbn;reflexivity].
-    eapply EPath_TPath in Htr1. cbn in Htr1. simpl_nl' Htr1. cbn in Htr1. eauto.
-  - eapply Tr_EPath in Htr2 as [s0 Htr2];[|cbn;reflexivity].
-    eapply EPath_TPath in Htr2. cbn in Htr2. simpl_nl' Htr2. cbn in Htr2. eauto.
-
-
-  Admitted.
-  
-(*  Lemma tr :
-    (Hsplit : join_andb
-             (map
-                (fun spl : Lab * Var =>
-                 let (s, x) := spl in
-                 uni s x &&
-                 join_andb
-                   (map (fun spl0 : Lab * Var => let (s0, x0) := spl0 in uni s0 x0)
-                        (preceding_loop_splits p s))) (splits p)) = true)
-      (HCuni : uni_concr uni ts)
-      (LC_lt : last_common (ne_map fst tq1) (ne_map fst tq2) (br, k))
-      (Hneq : q2 = q1)
-  decide' (i == I'). (* if the tag is the same there is a splitpoint *)
-  -- apply id in LC_lt as LC_lt'.
-     destruct LC_lt as [l1' [l2' [Hpost1 [Hpost2 [Hdisj [Hnin1 Hnin2]]]]]].
-     eapply last_common_splits in LC_lt'; eauto.
-     destruct LC_lt' as [x' HSsplit].
-     ++ 
-       eapply join_andb_true_iff in Hsplit; eauto.
-       conv_bool. [|apply in_or_app;left;eauto].
-       cbn in Hsplit. conv_bool. 
-       apply postfix_ex_unmapped_postfix' in Hpost1 as [l01 [s1' [Hpost1 Hposteq1]]].
-                apply postfix_ex_unmapped_postfix' in Hpost2 as [l02 [s2' [Hpost2 Hposteq2]]].
-                2,3: econstructor; apply zero.
-                eapply HCuni in Hsplit. all: cycle 1.
-                ** exact Hts1.
-                ** exact Hts2.
-                ** eapply prefix_incl;eauto. eapply prefix_trans.
-                   --- eapply prefix_nincl_prefix. eapply postfix_incl.
-                       eapply Hpost1. eapply In_rcons;eauto.
-                   --- subst tq1. rewrite <-nlcons_to_list. eapply prefix_nincl_prefix; eauto.
-                   --- left. reflexivity.
-                ** eapply prefix_incl;eauto. eapply prefix_trans.
-                   --- eapply prefix_nincl_prefix. eapply postfix_incl.
-                       eapply Hpost2. eapply In_rcons;eauto.
-                   --- subst tq2. rewrite <-nlcons_to_list. eapply prefix_nincl_prefix; eauto.
-                   --- left. reflexivity.
-                ** eapply splits_is_branch in HSsplit as HSbranch.
-                   assert (exists k, eff (S', i, s1') = Some k) as [k Hk] by eff_some_k.
-                   assert (exists k', eff (S', i, s2') = Some k') as [k' Hk'] by eff_some_k.
-                   eapply branch_eff_eq in Hsplit; eauto.
-                   subst l1' l2'.
-                   eapply not_same_step_disj_post with (q:=q); eauto.
-                   rewrite Hk, Hk'. cbn. 
-                   unfold option_fst. rewrite Hsplit. reflexivity.
-          -- (* if the tag is not the same there is loop_split of this splitpoint *)
-             (* TODO: adjust the proof to the switch of loop_split definition 
-                      and to the new transformer *)
-             apply id in LC_lt as LC_lt'.
-             eapply lc_loop_split with (i:=i) in LC_lt; cycle 1; eauto.
-             ++ subst tq1.
-                rewrite ne_map_nlcons. cbn. reflexivity.
-             ++ subst tq2;rewrite ne_map_nlcons; cbn; reflexivity.
-             ++ eapply Tr_EPath in Htr1 as [s0 Htr1]. eapply EPath_TPath in Htr1.
-                cbn in Htr1. econstructor; eauto. cbn. split; [apply Hqpred|].
-                eapply eff_eff_tag; eauto.                
-                subst tq1. simpl_nl. reflexivity.
-             ++ eapply Tr_EPath in Htr2 as [s0 Htr2]. eapply EPath_TPath in Htr2.
-                cbn in Htr2. econstructor; eauto. cbn. split; [apply Hqpred'|eauto].
-                eapply eff_eff_tag; eauto.
-                subst tq2. simpl_nl. reflexivity.
-             ++ destruct LC_lt as [X' HSsplit'].
-                destruct LC_lt' as [l1' [l2' [Hpost1 [Hpost2 [Hdisj [Hnin1 Hnin2]]]]]].
-                eapply join_andb_true_iff in Hsplit; [|apply in_or_app;right; eauto]. cbn in Hsplit.
-                conv_bool.                 
-                eapply postfix_ex_unmapped_postfix' in Hpost1 as [l01 [s1' [Hpost1 Hposteq1]]].
-                apply postfix_ex_unmapped_postfix' in Hpost2 as [l02 [s2' [Hpost2 Hposteq2]]].
-                2-5: eauto using zero, start_tag.
-                eapply HCuni in Hsplit. all: cycle 1.
-                ** exact Hts1.
-                ** exact Hts2.
-                ** eapply prefix_incl;eauto. eapply prefix_trans with (l2:=tq1).
-                   --- eapply prefix_nincl_prefix. eapply postfix_incl.
-                       eapply Hpost1. eapply In_rcons;eauto.
-                   --- subst tq1. rewrite <-nlcons_to_list. eapply prefix_nincl_prefix; eauto.
-                   --- left. reflexivity.
-                ** eapply prefix_incl;eauto. eapply prefix_trans with (l2:=tq2).
-                   --- eapply prefix_nincl_prefix. eapply postfix_incl.
-                       eapply Hpost2. eapply In_rcons;eauto.
-                   --- subst tq2. rewrite <-nlcons_to_list. eapply prefix_nincl_prefix; eauto.
-                   --- left. reflexivity.
-                ** eapply loop_splits_is_branch in HSsplit' as HSbranch.
-                   assert (exists k, eff (S', I', s1') = Some k) as [k Hk] by eff_some_k.
-                   (* because Tr ((p,i,s) ... (S',I',s')) *)
-                   assert (exists k', eff (S', I', s2') = Some k') as [k' Hk'] by eff_some_k.
-                   eapply branch_eff_eq in Hsplit; eauto.
-                   subst l1' l2'.
-                   eapply not_same_step_disj_post with (q:=q); eauto. 
-                   rewrite Hk,Hk'. cbn. rewrite Hsplit. reflexivity. *)
-   
+  symmetry in Hneq.
+  eapply lc_join_split in LC_lt as LC_join;eauto.
+  Unshelve. all:cycle 3. exact p. exact i.
+  - unfold last_common in LC_lt. destructH' LC_lt.
+    destruct l1',l2';cbn in *.
+    + (* q1 = br = q2 --> contradiction *) admit.
+    + (* since (br,k) = (q1,j1) & uniform, we have that (p,i) succeeds (br,k) thus
+         (p,i) ∈ l2, thus double occurence of the same instance in t2 --> contradiction *) admit.
+    + (* since (br,k) = (q2,j2) & uniform, we have that (p,i) succeeds (br,k) thus
+         (p,i) ∈ l1, thus double occurence of the same instance in t1 --> contradiction *) admit. 
+    + (* successor of br is the same because of uniformity and in l1' & l2', 
+         thus l1' & l2' are not disjoint --> contradiction *) admit.
+  - eapply Tr_EPath in Htr1; cbn;eauto. destruct Htr1 as [s01 Htr1]. eapply EPath_TPath in Htr1.
+    cbn in *. unfold TPath'. simpl_nl' Htr1. cbn in *. (* follows from Htr1 *) admit.
+  - (* follows from Htr2, if LC_join is adapted *) admit.
+  Admitted.   
   
   Lemma uni_correct :
-    forall uni upi unch ts,
-      sem_hyper (red_prod (red_prod (uni_concr uni) (upi_concr upi)) (lift (unch_concr unch))) ts ->
-      uni_concr (uni_trans uni upi unch) ts.
+    forall uni unch ts,
+      sem_hyper (red_prod (uni_concr uni) (lift (unch_concr unch))) ts ->
+      uni_concr (uni_trans uni unch) ts.
   Proof.
-    intros uni upi unch ts Hred.
+    intros uni unch ts Hred.
     unfold sem_hyper in Hred.
     destruct Hred as [ts' [Hconcr Hstep]].
     unfold uni_concr.
     intros t t' Hsem Hsem' x p i s s' HIn HIn' Htrans.
 
-    assert (upi_concr (upi_trans upi uni) ts) as HCupi. {
+(*    assert (upi_concr (upi_trans upi uni) ts) as HCupi. {
       apply upi_correct. 
       destruct Hconcr as [[_ Hhom] _].
       exists ts'; auto.
-    }
+    }*)
 
     assert (unch_concr (unch_trans unch) t) as HCunch. {
-      destruct Hconcr as [[_ _] Hunch].
+      destruct Hconcr as [_ Hunch].
       unfold lift in *; subst.
-      apply unch_correct. assumption.
+      apply unch_correct; [eapply root_no_pred'|]. assumption.
     } 
     
     assert (unch_concr (unch_trans unch) t') as HCunch'. {
-      destruct Hconcr as [[_ _] Hunch].
+      destruct Hconcr as [ _ Hunch].
       unfold lift in *; subst.
-      apply unch_correct. assumption.
+      apply unch_correct; [eapply root_no_pred'|]. assumption.
     }
 
-    destruct Hconcr as [[HCuni HCupi'] _].
+    destruct Hconcr as [HCuni  _].
 
     subst.
     unfold uni_trans in Htrans. 
@@ -313,24 +273,36 @@ Module Uniana.
         eapply prefix_cons_in in rp as rp'.
         assert (Prefix (`t1) (`t)) as pre_t.
         { rewrite Hteq1. cbn. econstructor. econstructor. }
-        eapply prefix_trans with (l2:=`t1) (l3:=`t) in rp; eauto.
-        apply prefix_cons_in in rp. eapply tag_inj in HIn; [| apply rp]. subst s0. eauto.
+        eapply prefix_trans with (l2:=`t1) (l3:=`t) in rp; eauto. 2:eapply root_no_pred'.
+        apply prefix_cons_in in rp. eapply tag_inj in HIn; [| eapply root_no_pred'| apply rp].
+        subst s0. eauto.
       + specialize (root_prefix t2) as [s0 rp]. apply root_start_tag in HIn as rst. subst i.
         eapply prefix_cons_in in rp as rp'.
         assert (Prefix (`t2) (`t')) as pre_t.
         { rewrite Hteq2. cbn. econstructor. econstructor. }
         eapply prefix_trans with (l2:=`t2) (l3:=`t') in rp; eauto.
-        apply prefix_cons_in in rp. eapply tag_inj in HIn'; [| apply rp]. subst s0. eauto.
+        apply prefix_cons_in in rp. eapply tag_inj in HIn'; [|eapply root_no_pred'| apply rp].
+        subst s0. eauto. eapply root_no_pred'.
     - conv_bool.
-      destruct Htrans as [Htrans | Hunch].
+      destruct Htrans as [[Htrans Hpred] | Hunch].
       (* The uni/hom case *)
-      + destruct Htrans as [[Hsplit Hpred] Hupi].
-        rewrite Hteq1 in HIn. rewrite Hteq2 in HIn'.
+      + rewrite Hteq1 in HIn. rewrite Hteq2 in HIn'.
         eapply in_pred_exists in HIn; try eassumption; [|setoid_rewrite <-Hteq1; exact (proj2_sig t)].
         eapply in_pred_exists in HIn'; try eassumption;[|setoid_rewrite <-Hteq2; exact (proj2_sig t')].
         destruct HIn as [q [j [r [HIn Hstep]]]].
         destruct HIn' as [q' [j' [r' [HIn' Hstep']]]].
-        assert (List.In q (preds p)) as Hqpred by (eauto using step_conf_implies_edge).
+        assert (q ∈ (preds p)) as Hqpred
+            by (eapply in_preds;eauto using step_conf_implies_edge,root_no_pred').
+
+        eapply prefix_in_list in HIn as Hpre1. destruct Hpre1 as [l1 Hpre1].
+          eapply prefix_in_list in HIn' as Hpre2. destruct Hpre2 as  [l2 Hpre2].
+          
+          rewrite nlcons_to_list in Hpre1.
+          eapply prefix_trace in Hpre1 as Htr1 ; [|eapply root_no_pred'|destruct t1; eauto].
+
+          rewrite nlcons_to_list in Hpre2.
+          eapply prefix_trace in Hpre2 as Htr2; [|eapply root_no_pred'|destruct t2;eauto].
+          simpl_nl' Hpre1. simpl_nl' Hpre2.
         cut (q' = q); intros; subst.
         * cut (j' = j); intros; subst.
           -- eapply (local_uni_corr (uni q) q j p i r r' s s'); try eassumption.
@@ -338,139 +310,17 @@ Module Uniana.
                 unfold uni_concr in HCuni .
                 eapply (HCuni _ _ Hts1 Hts2 x0 q j); eassumption.
              ** eapply join_andb_true_iff in Hpred; try eassumption.
-          -- (* unique preceding instances *)
-            eapply join_andb_true_iff in Hupi; try eassumption.
-            assert (p =/= q) by (symmetry; eauto using step_conf_implies_edge, no_self_loops).
-            symmetry.
-            eapply HCupi; [ eapply Hsem | eapply Hsem' | eassumption | | ].
-            1: rewrite Hteq1. 2: rewrite Hteq2.
-            all: cbn; rewrite nlcons_to_list; eapply precedes_step; eauto.
-            all: rewrite <-nlcons_necons.
-            ++ setoid_rewrite <-Hteq1. destruct t; cbn; eauto.
-            ++ setoid_rewrite <-Hteq2. destruct t'; cbn; eauto.
-        * (* disjoint paths! *)
-          clear Hpred HCunch HCunch' Hupi HCupi' HCupi.
-          eapply prefix_in_list in HIn as [l1 Hpre1].
-          eapply prefix_in_list in HIn' as [l2 Hpre2].
-          rewrite nlcons_to_list in Hpre1.
-          eapply prefix_trace in Hpre1 as Htr1; [|destruct t1; eauto].
-
-          eapply prefix_nlcons in Hpre1.
-          rewrite nlcons_to_list in Hpre2.
-          eapply prefix_trace in Hpre2 as Htr2; [|destruct t2;eauto].
-          eapply prefix_nlcons in Hpre2.
-          eapply disjoint with (t1:=t) (t2:=t'); eauto.
+          -- eapply uni_same_tag;eauto.
+             1,2: econstructor;eauto;simpl_nl;eauto.
+        * clear HCunch HCunch'.
+          eapply uni_same_lab with (t1:=t1) (t2:=t2); eauto.
           1,2: econstructor;eauto;simpl_nl;eauto.
-          1: setoid_rewrite Hteq1. 2: setoid_rewrite Hteq2.
-          1,2: simpl_nl; econstructor;eauto.
-          
-      (*destruct (q == q') as [ Heq | Hneq ]; [ eauto | exfalso ].
-          assert (In q' (preds p)) as Hqpred' by (eauto using step_conf_implies_edge).
-          
-          pose (tq1 := nlcons (q,j,r)     (prefix_nincl (q,j,r) (`t1))).
-          pose (tq2 := nlcons (q',j',r') (prefix_nincl (q',j',r') (`t2))).
-          assert (Tr tq1) as Htr1. {
-            eapply prefix_trace. subst tq1. rewrite <-nlcons_to_list.
-            eapply prefix_nincl_prefix.
-            eauto. destruct t1; eauto.
-          }
-          assert (Tr tq2) as Htr2. {
-            eapply prefix_trace. subst tq2. rewrite <-nlcons_to_list.
-            eapply prefix_nincl_prefix.
-            eauto. destruct t2;eauto.
-          }
-          assert (exists (si : Lab * Tag),
-                        last_common (ne_map fst tq1) (ne_map fst tq2) si) as [[S' I'] LC_lt].
-          {
-            eapply ne_last_common. repeat rewrite ne_back_map.
-            eapply ne_back_trace in Htr1 as [s1 Htr1].
-            eapply ne_back_trace in Htr2 as [s2 Htr2].
-            setoid_rewrite Htr1. setoid_rewrite Htr2. cbn;eauto.
-          } 
-          (**)
-          decide' (i == I'). (* if the tag is the same there is a splitpoint *)
-          -- apply id in LC_lt as LC_lt'.
-             destruct LC_lt as [l1' [l2' [Hpost1 [Hpost2 [Hdisj [Hnin1 Hnin2]]]]]].
-             eapply last_common_splits in LC_lt'; eauto.
-             destruct LC_lt' as [x' HSsplit].
-             ++ 
-               eapply join_andb_true_iff in Hsplit; eauto.
-               conv_bool. [|apply in_or_app;left;eauto].
-                cbn in Hsplit. conv_bool. 
-                apply postfix_ex_unmapped_postfix' in Hpost1 as [l01 [s1' [Hpost1 Hposteq1]]].
-                apply postfix_ex_unmapped_postfix' in Hpost2 as [l02 [s2' [Hpost2 Hposteq2]]].
-                2,3: econstructor; apply zero.
-                eapply HCuni in Hsplit. all: cycle 1.
-                ** exact Hts1.
-                ** exact Hts2.
-                ** eapply prefix_incl;eauto. eapply prefix_trans.
-                   --- eapply prefix_nincl_prefix. eapply postfix_incl.
-                       eapply Hpost1. eapply In_rcons;eauto.
-                   --- subst tq1. rewrite <-nlcons_to_list. eapply prefix_nincl_prefix; eauto.
-                   --- left. reflexivity.
-                ** eapply prefix_incl;eauto. eapply prefix_trans.
-                   --- eapply prefix_nincl_prefix. eapply postfix_incl.
-                       eapply Hpost2. eapply In_rcons;eauto.
-                   --- subst tq2. rewrite <-nlcons_to_list. eapply prefix_nincl_prefix; eauto.
-                   --- left. reflexivity.
-                ** eapply splits_is_branch in HSsplit as HSbranch.
-                   assert (exists k, eff (S', i, s1') = Some k) as [k Hk] by eff_some_k.
-                   assert (exists k', eff (S', i, s2') = Some k') as [k' Hk'] by eff_some_k.
-                   eapply branch_eff_eq in Hsplit; eauto.
-                   subst l1' l2'.
-                   eapply not_same_step_disj_post with (q:=q); eauto.
-                   rewrite Hk, Hk'. cbn. 
-                   unfold option_fst. rewrite Hsplit. reflexivity.
-          -- (* if the tag is not the same there is loop_split of this splitpoint *)
-             (* TODO: adjust the proof to the switch of loop_split definition 
-                      and to the new transformer *)
-             apply id in LC_lt as LC_lt'.
-             eapply lc_loop_split with (i:=i) in LC_lt; cycle 1; eauto.
-             ++ subst tq1.
-                rewrite ne_map_nlcons. cbn. reflexivity.
-             ++ subst tq2;rewrite ne_map_nlcons; cbn; reflexivity.
-             ++ eapply Tr_EPath in Htr1 as [s0 Htr1]. eapply EPath_TPath in Htr1.
-                cbn in Htr1. econstructor; eauto. cbn. split; [apply Hqpred|].
-                eapply eff_eff_tag; eauto.                
-                subst tq1. simpl_nl. reflexivity.
-             ++ eapply Tr_EPath in Htr2 as [s0 Htr2]. eapply EPath_TPath in Htr2.
-                cbn in Htr2. econstructor; eauto. cbn. split; [apply Hqpred'|eauto].
-                eapply eff_eff_tag; eauto.
-                subst tq2. simpl_nl. reflexivity.
-             ++ destruct LC_lt as [X' HSsplit'].
-                destruct LC_lt' as [l1' [l2' [Hpost1 [Hpost2 [Hdisj [Hnin1 Hnin2]]]]]].
-                eapply join_andb_true_iff in Hsplit; [|apply in_or_app;right; eauto]. cbn in Hsplit.
-                conv_bool.                 
-                eapply postfix_ex_unmapped_postfix' in Hpost1 as [l01 [s1' [Hpost1 Hposteq1]]].
-                apply postfix_ex_unmapped_postfix' in Hpost2 as [l02 [s2' [Hpost2 Hposteq2]]].
-                2-5: eauto using zero, start_tag.
-                eapply HCuni in Hsplit. all: cycle 1.
-                ** exact Hts1.
-                ** exact Hts2.
-                ** eapply prefix_incl;eauto. eapply prefix_trans with (l2:=tq1).
-                   --- eapply prefix_nincl_prefix. eapply postfix_incl.
-                       eapply Hpost1. eapply In_rcons;eauto.
-                   --- subst tq1. rewrite <-nlcons_to_list. eapply prefix_nincl_prefix; eauto.
-                   --- left. reflexivity.
-                ** eapply prefix_incl;eauto. eapply prefix_trans with (l2:=tq2).
-                   --- eapply prefix_nincl_prefix. eapply postfix_incl.
-                       eapply Hpost2. eapply In_rcons;eauto.
-                   --- subst tq2. rewrite <-nlcons_to_list. eapply prefix_nincl_prefix; eauto.
-                   --- left. reflexivity.
-                ** eapply loop_splits_is_branch in HSsplit' as HSbranch.
-                   assert (exists k, eff (S', I', s1') = Some k) as [k Hk] by eff_some_k.
-                   (* because Tr ((p,i,s) ... (S',I',s')) *)
-                   assert (exists k', eff (S', I', s2') = Some k') as [k' Hk'] by eff_some_k.
-                   eapply branch_eff_eq in Hsplit; eauto.
-                   subst l1' l2'.
-                   eapply not_same_step_disj_post with (q:=q); eauto. 
-                   rewrite Hk,Hk'. cbn. rewrite Hsplit. reflexivity. *)
       (* The unch case *)
       + rename Hunch into H.
         eapply join_orb_true_iff in H.
         destruct H as [u H].
         conv_bool.
-        destruct H as [Hunch [[Hneq' Huni] Hupi]].
+        destruct H as [Hunch [Hneq' Huni]].
         specialize (HCunch p i s u x HIn Hunch).
         specialize (HCunch' p i s' u x HIn' Hunch).
         destruct HCunch as [j [r [Hprec Heq]]]; try eassumption.
@@ -485,9 +335,9 @@ Module Uniana.
           -- rewrite <-nlcons_to_list. setoid_rewrite Hteq2 in Hprec'. apply Hprec'.
           -- rewrite <-nlcons_necons, <-Hteq2. destruct t'; eauto.
           -- cbn;eauto.
-        * symmetry. eapply (HCupi _ _ Hsem Hsem'); eauto.
-          Unshelve. all: exact (root,start_tag,zero).
-  Qed.
-
+        * symmetry. admit. 
+          (* eapply (HCupi _ _ Hsem Hsem'); eauto.*)
+  Admitted.
+  End uniana.
 
 End Uniana.
