Disjoint.v
@@ -12,20 +12,6 @@ Require Evaluation Util.
 Module Disjoint.
   Import Evaluation.Evaluation Util.
 
-  Parameter branch: Lab -> list Var.
-
-  Definition is_branch br x := x ∈ branch br.
-
-  Parameter val_true : Val -> bool.
-
-  Parameter branch_spec :
-    forall b, exists (d : list Val -> Lab), forall s, match (eff' (b, s)) with
-                                      | Some (q,_) => q = d (map s (branch b))
-                                      | None => True
-                                      end.
-  
-  Definition DisjointBranch `{redCFG} (s : Lab) (xl : list Var) (qt qf : Lab) (π ϕ : list Lab) :=
-    CPath s qt (π >: s) /\ CPath s qf (ϕ >: s) /\ branch s =' xl /\ Disjoint π ϕ.
 
   Parameter path_splits : forall `{redCFG}, Lab -> list (Lab * Lab * Lab).
 
@@ -35,7 +21,8 @@ Module Disjoint.
   Definition pl_split `{redCFG} (qh qe q1 q2 br : Lab) :=
       (exists π ϕ, CPath br qh (π >: q1 :>: br)
               /\ CPath br qe (ϕ >: q2 :>: br)
-              /\ Disjoint (tl (π :r: q1)) (tl (ϕ :r: q2))).
+              /\ q1 <> q2
+              /\ Disjoint (tl π) (tl ϕ)).
 
   Parameter path_splits_spec : forall `{redCFG} p q1 q2 br,
       pl_split p p q1 q2 br <->
@@ -62,16 +49,21 @@ Module Disjoint.
                                       \/ sp ∈ splits' br q').
 
   Definition splits_spec `{redCFG} := forall p sp, sp ∈ splits p
-                                              <-> sp ∈ path_splits__imp p
-                                                \/ exists br q q', (br,q,q') ∈ path_splits__imp p
-                                                                /\ (sp ∈ splits' br q
-                                                                   \/ sp ∈ splits' br q').
+                                              <-> sp ∈ path_splits__imp p (* usual split *)
+                                                \/ (exists h, let (p,_) := fst sp in
+                                                        (* lsplits of exited loops: *)
+                                                        exited h p /\ sp ∈ splits' h p)
+                                                \/ exists br q q',(br,q,q') ∈ path_splits__imp p
+                                                            (* loop_split of splitting heads *)
+                                                            /\ (sp ∈ splits' br q
+                                                               \/ sp ∈ splits' br q')
+  .
 
 
   Lemma lc_join_path_split_help1 (L : Type) (edge : L -> L -> bool) (x y : L) (l : list L)
     : @Path L edge x y (y :<: l >: x)
       -> exists z l', Path edge x y ((l' >: z) :>: x)
-                /\ (tl (l' :r: z)) ⊆ l.
+                /\ z ∈ l /\ (tl l') ⊆ l.
   Proof.
   Admitted.
 
@@ -182,13 +174,14 @@ Module Disjoint.
     let help := lc_join_path_split_help1 in eapply help in Hpath1;eauto; eapply help in Hpath2;eauto.
     destructH. destructH.
     exists z0, z, l'0, l'.
-    split_conj;eauto.
-    eapply disjoint_subset;eauto.
-    eapply lc_join_path_split_help2;eauto.
+    eapply lc_join_path_split_help2 in Hlc1;eauto.
+    - split_conj;eauto;[|eapply disjoint_subset;eauto]. eapply disjoint2;eauto.
+    - admit.
+    - admit.
   Admitted.
 
   Definition lc_disj_exit_lsplits_def (d : nat)
-    := forall `{redCFG} (s e q h : Lab) (i1 i2 j k : Tag) t1 t2 (n : nat)
+    := forall `{redCFG} (s e q h : Lab) (i1 i2 j k : Tag) (t1 t2 : ne_list Coord) (n : nat)
          (Hdep : d >= depth s - depth e)
          (Hlc : last_common t1 t2 (s,k))
          (Hhead : loop_head h)
@@ -200,7 +193,7 @@ Module Disjoint.
       exists (qq qq' : Lab) (xl : list Var), (s,qq,qq') ∈ loop_splits h e.
 
   Definition lc_disj_exits_lsplits_def (d : nat)
-    := forall `{redCFG} (s e1 e2 q1 q2 h : Lab) (i1 i2 j k : Tag) t1 t2 (n m : nat)
+    := forall `{redCFG} (s e1 e2 q1 q2 h : Lab) (i1 i2 j k : Tag) (t1 t2 : ne_list Coord) (n m : nat)
          (Hdep : d >= depth s - depth e1)
          (Hdep : d >= depth s - depth e2)
          (Hlc : last_common t1 t2 (s,k))
@@ -233,11 +226,13 @@ Module Disjoint.
   Qed.      
   
   Theorem lc_join_split `{redCFG} t1 t2 (p q1 q2 s : Lab) (i j1 j2 k : Tag)
-        (Hlc : last_common t1 t2 (s,k))
+          (* it is important to cons qj's in front of the t's *)
+        (Hlc : last_common ((q1,j1) :: t1) ((q2,j2) :: t2) (s,k))
         (Hneq : q1 <> q2 \/ j1 <> j2)
         (Hpath1 : TPath' ((p,i) :<: (q1,j1) :< t1))
         (Hpath2 : TPath' ((p,i) :<: (q2,j2) :< t2))
     : exists qq qq', (s,qq,qq') ∈ splits p.
+  Proof.
   Admitted.
 
   
