Unchanged.v
@@ -9,13 +9,13 @@ Module Unchanged.
   Import Evaluation.Evaluation Util.
   Open Scope prg.
 
-  Variable (edge a_edge : Lab -> Lab -> bool) (root : Lab) (C : redCFG edge root a_edge).
+  Section unch.
+  Context `{C : redCFG}.
     
   Variable root_no_pred' : forall p, p --> root -> False.
 
   Definition Unch := Lab -> Var -> set Lab.
 
-  Arguments Traces {_} {_} {_} {_}.
 
   Definition unch_concr (unch : Unch) : Traces :=
     fun t => forall to i s u x, In (to, i, s) (`t) ->
@@ -45,7 +45,8 @@ Module Unchanged.
     split.
     - unfold preds. induction all_lab; cbn; [contradiction|].
       destruct (edge a p) eqn:E;eauto.
-      + intro H. destruct H; subst;eauto.
+      + intro H. destruct H; subst;eauto. admit.
+      + admit.
     - admit.
   Admitted.
 
@@ -110,7 +111,6 @@ Module Unchanged.
       exists q, j, r. split; [ constructor |]; eauto.
   Qed.*)
 
-  Arguments sem_trace {_ _ _ _}.
 
   Lemma unch_correct :
     forall unch t,
@@ -127,8 +127,8 @@ Module Unchanged.
       simpl in Hunch. destruct Hunch; [ | firstorder ]. subst.      
       exists i, s. split; eauto. exists nil. split; [|econstructor].
       apply root_start_tag in Hin as rst. subst i.
-      assert (rp := root_prefix _ _ _ _ t). destruct rp as [s' rp].
-      apply prefix_cons_in in rp as rp'. eapply tag_inj with (s:=s) in rp'. 
+      assert (rp := root_prefix t). destruct rp as [s' rp].
+      apply prefix_cons_in in rp as rp'. eapply tag_inj with (s0:=s) in rp'. 
       subst s'. 1,3:assumption. all: eapply root_no_pred'.
     - assert (Hpred := Hin).
       rewrite H in Hpred.
@@ -144,160 +144,11 @@ Module Unchanged.
           edestruct Hred as [j' [r' [Hprec Heq]]]; eauto.
           exists j', r'. rewrite Heq.
           split; [|eauto using no_def_untouched]. rewrite H. eapply precedes_succ; eauto.
-          eapply root_no_pred'.
           rewrite <-H. destruct t; eauto.
       + clear - H. destruct t; cbn in H; inversion t; subst x.
         * congruence.
         * inversion H2. subst; eauto.
   Qed.
-  
-
-
-  
-
-  (*
-  Lemma unch_dom (u : Unch) x l l' :
-    set_In l (u l' x) -> forall q, is_def_lab x q -> forall (π : Path q l'), PathIn l π.
-  Proof.
-  Admitted.
-
-  Lemma unch_path_exist (u : Unch) x l l' r :
-    set_In l (u l' x) -> ~ set_In r (u l' x) -> exists (π : Path l l'), ~ PathIn r π.
-  Proof.
-  Admitted.
-    
-  Lemma front_and_join (u : Unch) x p :
-    Front u x p <-> is_def_lab x p \/ exists d d' q q' (π : Path d q) (π' : Path d' q'), is_def_lab x d /\
-                                                                                 is_def_lab x d' /\
-                                                                                 q --> p /\ q' --> p /\
-                                                                                 DisjPaths π π'.
-  Proof.
-    split; intros.
-    - induction H; [ left; assumption | right ].
-      eapply unch_path_exist in H6; try eassumption.
-      eapply unch_path_exist in H7; try eassumption.
-      destruct H6 as [π Hπ], H7 as [π' Hπ'].
-      specialize (unch_dom _ _ _ _ H4). intro Hdom.
-      specialize (unch_dom _ _ _ _ H5). intro Hdom'.
-      assert (Hdom := unch_dom _ _ _ _).
-      assert (DisjPaths π π'). {
-        unfold DisjPaths.
-        intros q.
-        split; intros.
-        - 
-
-      destruct IHFront1, IHFront2.
-      + exists l, r, l', r', π, π'.
-        do 4 (split; [ assumption |]).
-        unfold DisjPaths.
-        admit.
-      + 
-
-      assert  
-      (*
-      destruct IHFront1, IHFront2.
-      + exists l, r, l', r'.
-        eexists. eexists. 
-        do 4 (split; [ assumption |]).
-        admit.
-      +
-       *)
-      admit.
-    - admit.
-                           
-  *)
-
-  (* Paths *)
-
-
-  (*
-  Section Disj.
-    Variable unch : Unch.
-    Variable s t f : Lab.
-    Variable x xs : Var.
-    Variable Hst : s --> t.
-    Variable Hsf : s --> f.
-    Variable Hbr : branch s = Some (t, f, x, xs).
-    Variable Hfp : unch_lfp unch.
-
-    Lemma unch_split_is_on_path dl to (p : Path f to) :
-      unch to xs = Some dl ->
-      PathIn dl p.
-    Proof.
-      intros Hunch.
-      induction p.
-      - rename p into f. simpl.
-        assertl (Hbrspec := branch_spec_var s t f x xs Hbr).
-        destruct Hbrspec as [Hl [Hr _]].
-        destruct (unch_trans_res unch s f xs Hsf).
-        + rewrite unch_lfp_trans_eq in H; try eassumption.
-          rewrite Hunch in H. inject H. reflexivity.
-        + destruct H as [_ [H _]].  rewrite H in *; firstorder.
-      - rename from into f. rename p into q. simpl.
-        destruct (unch_trans_res unch q to xs e).
-        + rewrite unch_lfp_trans_eq in H; try eassumption.
-          rewrite Hunch in H. inject H. left. reflexivity.
-        + destruct H as [_ [_ [_ H]]].
-          rewrite unch_lfp_trans_eq in H; try eassumption.
-          rewrite H in Hunch. right. eauto.
-    Qed.
-    
-    Lemma unch_split_exists {to} (p : Path f to) :
-      exists dl, unch to xs = Some dl /\ PathIn dl p.
-    Proof.
-      induction p.
-      - rename p into f. simpl.
-        assert (Hbrspec := branch_spec_var s t f x xs Hbr).
-        destruct Hbrspec as [Hl [Hr _]].
-        destruct (unch_trans_res unch s f xs Hsf).
-        + rewrite unch_lfp_trans_eq in H; try eassumption.
-          exists f. split; [ eauto | reflexivity ].
-        + destruct H as [_ [H _]]. rewrite H in *; firstorder.
-      - rename from into f. rename p into q. simpl.
-        destruct (unch_trans_res unch q to xs e).
-        + rewrite unch_lfp_trans_eq in H; try eassumption.
-          exists to. split; eauto. 
-        + destruct H as [_ [_ [_ H]]].
-          rewrite unch_lfp_trans_eq in H; try eassumption.
-          destruct IHp as [dl [IHp Hin]]; try eassumption. rewrite IHp in H.
-          exists dl. eauto. 
-    Qed.
-
-    Variable l r : Lab.
-
-    Section PathsGiven.
-      Variable a : Path t l.
-      Variable b : Path f r.
-  
-      Lemma unch_disj_l :
-        disjoint a b ->
-        exists dl dr, unch l xs = Some dl /\ unch r xs = Some dr /\ dl =/= dr.
-      Proof.
-        intros Hdis.
-        unfold disjoint in Hdis.
-        destruct Hdis as [Hl Hr].
-        induction a as [t | t].
-        - destruct (branch_spec_var s t f x xs Hbr) as [Hdef _].
-          destruct (unch_trans_res unch s t xs Hst); rewrite unch_lfp_trans_eq in H; try eassumption.
-          + destruct (unch_split_exists b) as [dr [Hu Hp]].
-            exists t, dr. repeat split; try eassumption.
-            intro. eapply Hl. constructor. rewrite H0. assumption.
-          + destruct H as [_ [H _]]. rewrite Hdef in H. firstorder.
-        - rename p0 into b', p into l.
-          destruct IHp; try eassumption.
-          + intros. apply Hl. simpl. auto.
-          + intros. apply Hr in H. contradict H. simpl. auto.
-          + destruct H as [dr [Hul [Hur Hneq]]].
-            destruct (unch_trans_res unch l to xs e); rewrite unch_lfp_trans_eq in H; try eassumption.
-            * exists to, dr. repeat split; eauto. 
-              intro. eapply (Hl to). simpl. left. reflexivity. eapply unch_split_is_on_path. auto.
-              rewrite H0. eassumption.
-            * destruct H as [_ [_ [_ H]]].
-              rewrite H. eauto.
-      Qed.
-
-*)
-
-
-
+  End unch.
 End Unchanged.
+
